new algo for au

src/MC_algo_sandbox02.v
@@ -93,7 +93,121 @@ Defined.
 Definition usefull3: forall m n:nat, m <= n -> m - 1 <= n - 1.
 lia.
 Defined. 
-Theorem F1AU: forall st: state model_triangle, 
+
+
+
+Ltac SOLVE_AU STATE_SIZE init_l := 
+let solve_AU max_of_state :=
+  let path_pi := fresh "path_pi" in
+  intro path_pi;
+  let is_path_pi := fresh "is_path_pi" in
+  intro is_path_pi;
+  let first_state:= fresh "first_state" in
+  intro first_state;
+  compute;
+  let rec sol_AU n :=
+  tryif (let h:= fresh "h" in assert(h: n + 1 <= max_of_state); [progress auto | auto])
+  then
+    (eexists n (*n*); 
+    [
+      auto;
+        let m := fresh "m" in
+        let le_m := fresh "le_m" in
+        intro m;
+        intro le_m;
+        repeat split;
+        (
+          let pre := fresh "pre" in
+          intro pre;
+          let rec solve_rec m le_m pre := 
+            apply usefull in le_m; compute in le_m;
+            let first_case := fresh "first_case" in
+            let second_case := fresh "second_case" in
+            destruct le_m as [ first_case | second_case]; 
+            [> 
+            (apply usefull2 in first_case;
+              rewrite first_case in pre;
+              rewrite init_l in first_state;
+              rewrite first_state in pre; discriminate) +
+              (apply usefull2 in first_case;
+              rewrite first_case in pre;
+              rewrite init_l in first_state;
+              pose proof (is_path_pi 0) as is_path_pi_0; compute in is_path_pi_0;
+              repeat let a := fresh "is_path_pi_0" in
+              destruct is_path_pi_0 as (a&is_path_pi_0);
+              try ((apply a in first_state)+(apply is_path_pi_0 in first_state);rewrite first_state in pre; discriminate) )
+              
+            | 
+              lia +  
+              (solve_rec (m-1) second_case pre) + auto
+            ]
+          in
+          (solve_rec m le_m pre)
+        )
+        
+      |
+        compute;
+        rewrite init_l in first_state ;  
+        repeat split;
+        let pre := fresh "pre" in
+        let H := fresh "H" in
+        intro pre;
+        (
+          
+  
+            let rec progress_in_edges m first_state :=
+              
+              ((
+                let is_path_pi_0:= fresh "is_path_pi_0" 
+                in
+                pose proof (is_path_pi m) as is_path_pi_0; 
+                compute in is_path_pi_0; 
+                repeat (
+                  let a := fresh "is_path_pi_0" in
+                  destruct is_path_pi_0 as (a&is_path_pi_0);
+                  (apply a in first_state) + (apply is_path_pi_0 in first_state)
+                );
+                rewrite first_state in pre; discriminate
+                ;
+                try (apply is_path_pi_0 in first_state;rewrite first_state in pre; discriminate)
+              ) 
+              +
+              (
+                (
+                  let is_path_pi_0:= fresh "is_path_pi_0" 
+                  in
+                  pose proof (is_path_pi m) as is_path_pi_0; 
+                  compute in is_path_pi_0; 
+                  repeat (
+                    let a := fresh "is_path_pi_0" in
+                    destruct is_path_pi_0 as (a&is_path_pi_0);
+                    (apply a in first_state) + (apply is_path_pi_0 in first_state)
+                  );
+                  tryif (let h:= fresh "h" in assert(h: m+1 < n); [progress auto| auto])
+                  then
+                  progress_in_edges (m+1) first_state 
+                  else 
+                  fail "progress_in_edges: with" m "and 1"
+                )
+              ))
+            in
+            progress_in_edges 0 first_state
+        )
+    ])
+    +
+    sol_AU (n + 1)
+  else 
+  fail "solve_AU: with" n
+  in
+  sol_AU 0
+in
+(* auto. *)
+solve_AU STATE_SIZE.
+
+
+
+
+  Theorem F1AU: forall st: state model_triangle, 
 (init model_triangle) st -> 
 satisfies (model_triangle) (fAU (fV 1)(fV 0)) st.
 Proof.
@@ -101,107 +215,114 @@ Proof.
   intro st_l.
   let init_l := fresh "init_l" in
   intro init_l. compute in init_l.
-  let path_pi := fresh "path_pi" in
-  intro path_pi.
-  let is_path_pi := fresh "is_path_pi" in
-  intro is_path_pi.
-  let first_state:= fresh "first_state" in
-  intro first_state.
-  compute.
-
   
-  (* let solve_AU n path_pi is_path_pi first_state := 
+  let solve_AU max_of_state :=
+    let path_pi := fresh "path_pi" in
+    intro path_pi;
+    let is_path_pi := fresh "is_path_pi" in
+    intro is_path_pi;
+    let first_state:= fresh "first_state" in
+    intro first_state;
+    compute;
+    let rec sol_AU n :=
+    tryif (let h:= fresh "h" in assert(h: n + 1 <= max_of_state); [progress auto | auto])
+    then
+      (eexists n (*n*); 
+      [
+        auto;
+          let m := fresh "m" in
+          let le_m := fresh "le_m" in
+          intro m;
+          intro le_m;
+          repeat split;
+          (
+            let pre := fresh "pre" in
+            intro pre;
+            let rec solve_rec m le_m pre := 
+              apply usefull in le_m; compute in le_m;
+              let first_case := fresh "first_case" in
+              let second_case := fresh "second_case" in
+              destruct le_m as [ first_case | second_case]; 
+              [> 
+              (apply usefull2 in first_case;
+                rewrite first_case in pre;
+                rewrite init_l in first_state;
+                rewrite first_state in pre; discriminate) +
+                (apply usefull2 in first_case;
+                rewrite first_case in pre;
+                rewrite init_l in first_state;
+                pose proof (is_path_pi 0) as is_path_pi_0; compute in is_path_pi_0;
+                repeat let a := fresh "is_path_pi_0" in
+                destruct is_path_pi_0 as (a&is_path_pi_0);
+                try (apply is_path_pi_0 in first_state;rewrite first_state in pre; discriminate) )
+                
+              | 
+                lia +  
+                (solve_rec (m-1) second_case pre) + auto
+              ]
+            in
+            (solve_rec m le_m pre)
+          )
+          
+        |
+          compute;
+          rewrite init_l in first_state ;  
+          repeat split;
+          let pre := fresh "pre" in
+          let H := fresh "H" in
+          intro pre;
+          (
+            
     
-    eexists n;
-    
-    [
-      auto;
-      let m := fresh "m" in
-      let le_m := fresh "le_m" in
-      intro m;
-      intro le_m;
-      repeat split
-      ;
-      (
-        let pre := fresh "pre" in
-        
-        let first_case := fresh "first_case" in
-        let second_case := fresh "second_case" in
-
-        intro pre;
-        let rec solve_pattern le_m := 
-          apply usefull in le_m; compute in le_m;
-          destruct le_m as [ first_case | second_case];
-          tryif [> lia|lia ] 
-          then 
-          [>
-            apply usefull2 in first_case;
-              rewrite first_case in pre;
-              rewrite init_l in first_state;
-              rewrite first_state in pre; discriminate
-            |
-            auto
-          ]
-          else 
-          [>
-            apply usefull2 in first_case;
-            rewrite first_case in pre;
-            rewrite init_l in first_state;
-            pose proof (is_path_pi 0) as is_path_pi_0; compute in is_path_pi_0;
-            repeat let a := fresh "is_path_pi_0" in
-            destruct is_path_pi_0 as (a&is_path_pi_0);
-            try (apply is_path_pi_0 in first_state;rewrite first_state in pre; discriminate)
-            |
-            solve_pattern second_case
-            ]
-          (* [
-            apply usefull2 in first_case;
-            rewrite first_case in pre;
-            rewrite init_l in first_state;
-            pose proof (is_path_pi 0) as is_path_pi_0; compute in is_path_pi_0;
-            repeat let a := fresh "is_path_pi_0" in
-            destruct is_path_pi_0 as (a&is_path_pi_0);
-            try (apply is_path_pi_0 in first_state;rewrite first_state in pre; discriminate)
-          |
-            apply usefull in second_case; compute in second_case;
-            destruct second_case as [ first_case | second_case]
-            ;[
-              apply usefull2 in first_case;
-              rewrite first_case in pre;
-              rewrite init_l in first_state;
-              rewrite first_state in pre; discriminate
-              (* apply usefull2 in first_case;
-            rewrite first_case in pre;
-            rewrite init_l in first_state;
-            pose proof (is_path_pi 0) as is_path_pi_0; compute in is_path_pi_0;
-            repeat let a := fresh "is_path_pi_0" in
-            destruct is_path_pi_0 as (a&is_path_pi_0);
-            try (apply is_path_pi_0 in first_state;rewrite first_state in pre; discriminate) *)
-              |
-              lia]
-          ] *)
-        in
-        solve_pattern le_m
-      )
-      | let solve_m :=
-      let progress_in_edges m first_state :=
-        let is_path_pi_0:= fresh "is_path_pi_0" in
-        pose proof (is_path_pi m) as is_path_pi_0; compute in is_path_pi_0; 
-        repeat let a := fresh "is_path_pi_0" in
-        destruct is_path_pi_0 as (a&is_path_pi_0);
-        (apply a in first_state) + (apply is_path_pi_0 in first_state)
-      in
-      intro pre;
-      rewrite init_l in first_state;
-      progress_in_edges 0 first_state;
-      progress_in_edges 1 first_state;
-      rewrite first_state in pre; discriminate 
-    in 
-    repeat split;solve_m
-    ]
-  in *)
-  (* solve_AU 2 path_pi is_path_pi first_state. *)
-  eexists 2 (*n*); 
+              let rec progress_in_edges m first_state :=
+                
+                ((
+                  let is_path_pi_0:= fresh "is_path_pi_0" 
+                  in
+                  pose proof (is_path_pi m) as is_path_pi_0; 
+                  compute in is_path_pi_0; 
+                  repeat (
+                    let a := fresh "is_path_pi_0" in
+                    destruct is_path_pi_0 as (a&is_path_pi_0);
+                    (apply a in first_state) + (apply is_path_pi_0 in first_state)
+                  );
+                  rewrite first_state in pre; discriminate
+                  ;
+                  try (apply is_path_pi_0 in first_state;rewrite first_state in pre; discriminate)
+                ) 
+                +
+                (
+                  (
+                    let is_path_pi_0:= fresh "is_path_pi_0" 
+                    in
+                    pose proof (is_path_pi m) as is_path_pi_0; 
+                    compute in is_path_pi_0; 
+                    repeat (
+                      let a := fresh "is_path_pi_0" in
+                      destruct is_path_pi_0 as (a&is_path_pi_0);
+                      (apply a in first_state) + (apply is_path_pi_0 in first_state)
+                    );
+                    tryif (let h:= fresh "h" in assert(h: m+1 < n); [progress auto| auto])
+                    then
+                    progress_in_edges (m+1) first_state 
+                    else 
+                    fail "progress_in_edges: with" m "and 1"
+                  )
+                ))
+              in
+              progress_in_edges 0 first_state
+          )
+      ])
+      +
+      sol_AU (n + 1)
+    else 
+    fail "solve_AU: with" n
+    in
+    sol_AU 0
+  in
+  (* auto. *)
+  SOLVE_AU 3 init_l.
+  (* eexists 2 (*n*); 
   [
     auto;
       let m := fresh "m" in
@@ -233,187 +354,214 @@ Proof.
           | 
             lia +  
             (solve_rec (m-1) second_case pre) + auto
-          ] 
-
-          
+          ]
         in
         (solve_rec m le_m pre)
       )
       
     |
-    (* let progress_in_edges m first_state :=
-        let is_path_pi_0:= fresh "is_path_pi_0" in
-        pose proof (is_path_pi m) as is_path_pi_0; compute in is_path_pi_0; 
-        repeat let a := fresh "is_path_pi_0" in
-        destruct is_path_pi_0 as (a&is_path_pi_0);
-        (apply a in first_state) + (apply is_path_pi_0 in first_state)
-      in *)
       
-    rewrite init_l in first_state ;  
-    repeat split;
-    let pre := fresh "pre" in
-    let H := fresh "H" in
-    intro pre;
+      rewrite init_l in first_state ;  
+      repeat split;
+      let pre := fresh "pre" in
+      let H := fresh "H" in
+      intro pre;
+      (
+        
+
+          let rec progress_in_edges m first_state :=
+            
+            ((
+              let is_path_pi_0:= fresh "is_path_pi_0" 
+              in
+              pose proof (is_path_pi m) as is_path_pi_0; 
+              compute in is_path_pi_0; 
+              repeat (
+                let a := fresh "is_path_pi_0" in
+                destruct is_path_pi_0 as (a&is_path_pi_0);
+                (apply a in first_state) + (apply is_path_pi_0 in first_state)
+              );
+              rewrite first_state in pre; 
+              discriminate;
+              try (apply is_path_pi_0 in first_state;rewrite first_state in pre; discriminate)
+            ) 
+            +
+            (
+              (
+                let is_path_pi_0:= fresh "is_path_pi_0" 
+                in
+                pose proof (is_path_pi m) as is_path_pi_0; 
+                compute in is_path_pi_0; 
+                repeat (
+                  let a := fresh "is_path_pi_0" in
+                  destruct is_path_pi_0 as (a&is_path_pi_0);
+                  (apply a in first_state) + (apply is_path_pi_0 in first_state)
+                );
+                tryif (let h:= fresh "h" in assert(h: m+1 < 2); [progress auto| auto])
+                then
+                progress_in_edges (m+1) first_state 
+                else 
+                fail "progress_in_edges: with" m "and 1"
+              )
+            ))
+          in
+          progress_in_edges 0 first_state
+      )
+  ]. *)
+Defined.
+
+
+
+Definition from_trans_to_Prop2{A}(list_connections: list (A*A)): A -> A -> Prop :=
+(fun s1 s2 =>
+  let fix make_prop (list_connections: list (A*A)):Prop :=
+    match list_connections with 
+    | (b1,b2)::nil => (s1 = b1 /\ (s2 = b2))
+    | (b1,b2)::tail => (s1 = b1 /\ (s2 = b2)) \/ (make_prop tail)
+    | nil => False
+    end in 
+  make_prop list_connections).
+(* Testing AU tactic *)
+Inductive   sq : Set :=  one_sq | two_sq | three_sq | four_sq.
+Definition  trans_sq := fun x x0 : sq =>
+(x = three_sq -> x0 = four_sq) /\
+(x = four_sq -> ((x0 = one_sq) \/ (x0 = two_sq))) /\
+(x = two_sq -> x0 = two_sq) /\ (x = one_sq -> x0 = one_sq).
+  (* from_trans_to_Prop [(three_sq, four_sq);(four_sq, one_sq);(four_sq, two_sq); (two_sq, two_sq); (one_sq, one_sq)]. *)
+Compute trans_sq.
+Definition  label_sq := from_label_to_Prop [(one_sq, 0); (two_sq, 0); (three_sq,1); (four_sq, 1)].
+
+Definition  serial_sq: forall w:sq, exists (v:sq), trans_sq w v.
+intro; case w;[eexists one_sq | eexists two_sq | eexists four_sq | eexists one_sq].
+compute. repeat split; intro; discriminate.
+compute. repeat split; intro; discriminate.
+compute. repeat split; intro; discriminate.
+compute. repeat split; intro. try discriminate. left. auto. discriminate.
+Defined.
+
+
+Definition init_sq := from_init_to_Prop [three_sq].
+Definition model_sq: sts :=  {| 
+  state   := sq; 
+  trans   := trans_sq; 
+  init    := init_sq; 
+  label   := label_sq; 
+  serial  := serial_sq 
+|}.
+Ltac test_ltb_m_n m n:=
+assert (m < n);progress auto
+.
+
+Ltac SOLVE_AU2 n STATE_SIZE init_l := 
+let solve_AU max_of_state :=
+  let path_pi := fresh "path_pi" in
+  intro path_pi;
+  let is_path_pi := fresh "is_path_pi" in
+  intro is_path_pi;
+  let first_state:= fresh "first_state" in
+  intro first_state;
+  compute;
+  let rec sol_AU n :=
+  tryif (let h:= fresh "h" in assert(h: n <= max_of_state); [progress auto | auto])
+  then
     (
-      let progress_rec m first_state :=
-        let progress_in_edges m first_state :=
-          let is_path_pi_0:= fresh "is_path_pi_0" in
-          pose proof (is_path_pi m) as is_path_pi_0; compute in is_path_pi_0; 
-          repeat let a := fresh "is_path_pi_0" in
-          destruct is_path_pi_0 as (a&is_path_pi_0);
-          (apply a in first_state) + (apply is_path_pi_0 in first_state)
-        in
-        let rec body m first_state := 
-        (progress_in_edges m first_state; rewrite first_state in pre;discriminate)
-        +
-        (progress_in_edges m first_state;body (m+1) first_state)
-        in
-        body m first_state;
-        try (apply is_path_pi_0 in first_state;rewrite first_state in pre; discriminate)
-      in 
-      progress_rec 0 first_state
-      
-    )
-  ].
-Defined.
-
-
-
-
-
-
-
-
-
-
-
-
-
-
-
-
-
-  {
-    let m := fresh "m" in
-    intro m.
-    let le_m := fresh "le_m" in
-    intro le_m.
-    repeat split.
-    {
-      intro pre; apply usefull in le_m; compute in le_m.
-      let first_case := fresh "first_case" in
-      let second_case := fresh "second_case" in
-      destruct le_m as [ first_case | second_case];
+      eexists n (*n*); 
       [
-        apply usefull2 in first_case;
-        rewrite first_case in pre;
-        rewrite init_l in first_state;
-        pose proof (is_path_pi 0) as is_path_pi_0; compute in is_path_pi_0;
-        repeat let a := fresh "is_path_pi_0" in
-        destruct is_path_pi_0 as (a&is_path_pi_0);
-        try (apply is_path_pi_0 in first_state;rewrite first_state in pre; discriminate)
-      |
-        apply usefull in second_case;
-        destruct second_case as [ first_case | second_case]
-        ;[
-          apply usefull2 in first_case;
-          rewrite first_case in pre;
-          rewrite init_l in first_state;
-          rewrite first_state in pre; discriminate
-          
-          |
-          lia]
-      ].
-    } 
-  }{
-    (* repeat split; intro pre. *)
-    (* proof that m=2 is ok *)
-    let solve_m :=
-      let progress_in_edges m first_state :=
-        let is_path_pi_0:= fresh "is_path_pi_0" in
-        pose proof (is_path_pi m) as is_path_pi_0; compute in is_path_pi_0; 
-        repeat let a := fresh "is_path_pi_0" in
-        destruct is_path_pi_0 as (a&is_path_pi_0);
-        (apply a in first_state) + (apply is_path_pi_0 in first_state)
+          auto;
+          let m := fresh "m" in
+          let le_m := fresh "le_m" in
+          intro m;
+          intro le_m;
+          repeat split;
+          (
+            let pre := fresh "pre" in
+            intro pre;
+            let rec solve_rec m le_m pre := 
+              apply usefull in le_m; compute in le_m;
+              let first_case := fresh "first_case" in
+              let second_case := fresh "second_case" in
+              destruct le_m as [ first_case | second_case]; 
+              [> 
+              (apply usefull2 in first_case;
+                rewrite first_case in pre;
+                rewrite init_l in first_state;
+                rewrite first_state in pre; discriminate) +
+                (apply usefull2 in first_case;
+                rewrite first_case in pre;
+                rewrite init_l in first_state;
+                pose proof (is_path_pi 0) as is_path_pi_0; compute in is_path_pi_0;
+                repeat let a := fresh "is_path_pi_0" in
+                destruct is_path_pi_0 as (a&is_path_pi_0);
+                try ((apply a in first_state)+(apply is_path_pi_0 in first_state);rewrite first_state in pre; discriminate) )
+                
+              | 
+                lia +  
+                (solve_rec (m-1) second_case pre) + auto
+              ]
+            in
+            (solve_rec m le_m pre)
+          )
+        |
+        let progress_in_edges n :=
+          compute;
+          rewrite init_l in first_state ;  
+          repeat split;
+          let pre := fresh "pre" in
+          intro pre;
+          let rec through_edge m first_state := 
+            (
+              lazymatch goal with 
+              | first_state: ?K \/ ?L |- _ => (destruct first_state as [first_state|first_state])
+              | first_state: _ |- _ => idtac
+              end
+            );
+            (let is_path_pi_0:= fresh "is_path_pi_0" in
+            pose proof (is_path_pi m) as is_path_pi_0; 
+            compute in is_path_pi_0; 
+            repeat (
+              let a := fresh "is_path_pi_0" in
+              destruct is_path_pi_0 as (a&is_path_pi_0);
+              ((apply a in first_state) + (apply is_path_pi_0 in first_state))
+            ));
+            (
+              lazymatch goal with 
+              | first_state: ?K \/ ?L |- _ => (destruct first_state as [first_state|first_state])
+              | first_state: _ |- _ => idtac
+              end
+            );
+            ((rewrite first_state in pre; 
+            discriminate)
+            +
+            (
+              tryif (let h:= fresh "h" in assert(h: m + 1 <= n); [progress auto | auto])
+              then through_edge (m+1) first_state
+              else idtac
+              )
+            )
+          in
+          through_edge 0 first_state
       in
-      intro pre;
-      rewrite init_l in first_state;
-      progress_in_edges 0 first_state;
-      progress_in_edges 1 first_state;
-      rewrite first_state in pre; discriminate 
-    in 
-    repeat split;solve_m.
-  } Defined.
+      progress_in_edges max_of_state
+      ]
+    )
+    +
+    sol_AU (n + 1)
+  else 
+  fail "solve_AU: with" n
+  in
+  sol_AU n
+in
+solve_AU n.
 
 
-    { (*case k < m*)
-        rewrite H in pre.
-        rewrite init_l in first_state.
-        pose proof (is_path_pi 0) as is_path_pi_0. compute in is_path_pi_0. 
-        repeat let a := fresh "is_path_pi_0" in
-        destruct is_path_pi_0 as (a&is_path_pi_0); 
-        try (apply is_path_pi_0 in first_state;rewrite first_state in pre; discriminate).
-      }
-      {  (*case 0 = m*)
-        rewrite H in pre.
-        rewrite init_l in first_state.
-        rewrite first_state in pre. discriminate.
-      }
-
-  }
-      
-        rewrite first_case in pre.
-        rewrite init_l in first_state.
-        pose proof (is_path_pi 0) as is_path_pi_0. compute in is_path_pi_0. 
-        repeat let a := fresh "is_path_pi_0" in
-        destruct is_path_pi_0 as (a&is_path_pi_0); 
-        try (apply is_path_pi_0 in first_state;rewrite first_state in pre; discriminate).
-      
-        apply usefull in H.
-        compute in H.
-        apply usefull2 in H.
-        rewrite H in pre.
-        rewrite init_l in first_state.
-        pose proof (is_path_pi 0) as is_path_pi_0. compute in is_path_pi_0. 
-        repeat let a := fresh "is_path_pi_0" in
-        destruct is_path_pi_0 as (a&is_path_pi_0); 
-        try (apply is_path_pi_0 in first_state;rewrite first_state in pre; discriminate).
-
-      }
-
-
-      { (*case k < m*)
-        rewrite H in pre.
-        rewrite init_l in first_state.
-        pose proof (is_path_pi 0) as is_path_pi_0. compute in is_path_pi_0. 
-        repeat let a := fresh "is_path_pi_0" in
-        destruct is_path_pi_0 as (a&is_path_pi_0); 
-        try (apply is_path_pi_0 in first_state;rewrite first_state in pre; discriminate).
-      }
-      {  (*case 0 = m*)
-        rewrite H in pre.
-        rewrite init_l in first_state.
-        rewrite first_state in pre. discriminate.
-      }
-    }
-  }
-  {
-    (* proof that m=2 is ok *)
-    let solve_m :=
-      let progress_in_edges m first_state :=
-        let is_path_pi_0:= fresh "is_path_pi_0" in
-        pose proof (is_path_pi m) as is_path_pi_0; compute in is_path_pi_0; 
-        repeat let a := fresh "is_path_pi_0" in
-        destruct is_path_pi_0 as (a&is_path_pi_0);
-        (apply a in first_state) + (apply is_path_pi_0 in first_state)
-      in
-      intro pre;
-      rewrite init_l in first_state;
-      progress_in_edges 0 first_state;
-      progress_in_edges 1 first_state;
-      rewrite first_state in pre; discriminate 
-    in 
-    repeat split;solve_m.
-  }
+(* try (destruct first_state; [auto|auto]). *)
+Theorem F2AU: forall st: state model_sq, 
+(init model_sq) st -> 
+satisfies (model_sq) (fAU (fV 1)(fV 0)) st.
+Proof.
+  let st_l := fresh "st_l" in
+  intro st_l.
+  let init_l := fresh "init_l" in
+  intro init_l. compute in init_l.
+  SOLVE_AU2 2 4 init_l.
 Defined.
-  
